tests/lean/StepBy.lean
@@ -57,7 +57,7 @@ def test_step_by_1 : Result Unit := do
   massert b
 
 /- Unit test for [step_by::test_step_by_1] -/
-#assert ((test_step_by_1 ).is_ok ())
+#assert (test_step_by_1).reducesTo ()
 
 /-- [step_by::test_step_by_2]:
     Source: 'tests/src/step_by.rs', lines 21:0-28:1
@@ -92,7 +92,7 @@ def test_step_by_2 : Result Unit := do
   massert b
 
 /- Unit test for [step_by::test_step_by_2] -/
-#assert ((test_step_by_2 ).is_ok ())
+#assert (test_step_by_2).reducesTo ()
 
 /-- [step_by::test_step_by_3]:
     Source: 'tests/src/step_by.rs', lines 32:0-39:1
@@ -127,7 +127,7 @@ def test_step_by_3 : Result Unit := do
   massert b
 
 /- Unit test for [step_by::test_step_by_3] -/
-#assert ((test_step_by_3 ).is_ok ())
+#assert (test_step_by_3).reducesTo ()
 
 /-- [step_by::test_step_by_larger_than_len]:
     Source: 'tests/src/step_by.rs', lines 43:0-48:1
@@ -150,7 +150,7 @@ def test_step_by_larger_than_len : Result Unit := do
   massert b
 
 /- Unit test for [step_by::test_step_by_larger_than_len] -/
-#assert ((test_step_by_larger_than_len ).is_ok ())
+#assert (test_step_by_larger_than_len).reducesTo ()
 
 /-- [step_by::test_step_by_empty]:
     Source: 'tests/src/step_by.rs', lines 52:0-56:1
@@ -168,7 +168,7 @@ def test_step_by_empty : Result Unit := do
   massert b
 
 /- Unit test for [step_by::test_step_by_empty] -/
-#assert ((test_step_by_empty ).is_ok ())
+#assert (test_step_by_empty).reducesTo ()
 
 /-- [step_by::test_step_by_single]:
     Source: 'tests/src/step_by.rs', lines 60:0-65:1
@@ -191,7 +191,7 @@ def test_step_by_single : Result Unit := do
   massert b
 
 /- Unit test for [step_by::test_step_by_single] -/
-#assert ((test_step_by_single ).is_ok ())
+#assert (test_step_by_single).reducesTo ()
 
 /-- [step_by::test_step_by_single_step_2]:
     Source: 'tests/src/step_by.rs', lines 69:0-74:1
@@ -214,7 +214,7 @@ def test_step_by_single_step_2 : Result Unit := do
   massert b
 
 /- Unit test for [step_by::test_step_by_single_step_2] -/
-#assert ((test_step_by_single_step_2 ).is_ok ())
+#assert (test_step_by_single_step_2).reducesTo ()
 
 /-- [step_by::test_step_by_eq_len]:
     Source: 'tests/src/step_by.rs', lines 78:0-83:1
@@ -237,7 +237,7 @@ def test_step_by_eq_len : Result Unit := do
   massert b
 
 /- Unit test for [step_by::test_step_by_eq_len] -/
-#assert ((test_step_by_eq_len ).is_ok ())
+#assert (test_step_by_eq_len).reducesTo ()
 
 /-- [step_by::test_step_by_len_minus_1]:
     Source: 'tests/src/step_by.rs', lines 87:0-93:1
@@ -265,7 +265,7 @@ def test_step_by_len_minus_1 : Result Unit := do
   massert b
 
 /- Unit test for [step_by::test_step_by_len_minus_1] -/
-#assert ((test_step_by_len_minus_1 ).is_ok ())
+#assert (test_step_by_len_minus_1).reducesTo ()
 
 /-- [step_by::test_step_by_two_elements]:
     Source: 'tests/src/step_by.rs', lines 97:0-102:1
@@ -288,7 +288,7 @@ def test_step_by_two_elements : Result Unit := do
   massert b
 
 /- Unit test for [step_by::test_step_by_two_elements] -/
-#assert ((test_step_by_two_elements ).is_ok ())
+#assert (test_step_by_two_elements).reducesTo ()
 
 /-- [step_by::test_step_by_4_on_longer]:
     Source: 'tests/src/step_by.rs', lines 106:0-113:1
@@ -326,6 +326,6 @@ def test_step_by_4_on_longer : Result Unit := do
   massert b
 
 /- Unit test for [step_by::test_step_by_4_on_longer] -/
-#assert ((test_step_by_4_on_longer ).is_ok ())
+#assert (test_step_by_4_on_longer).reducesTo ()
 
 end step_by
